enviar trabalho

cp-basic/cp.dfy
@@ -16,14 +16,58 @@ method ArrayFromSeq<A>(s: seq<A>) returns (a: array<A>)
 method {:main} Main(ghost env: HostEnvironment?)
   requires env != null && env.Valid() && env.ok.ok();
   requires |env.constants.CommandLineArgs()|>= 3
+  requires env.constants.CommandLineArgs()[1] in env.files.state()
   modifies env.ok
-  modifies env.files
+  modifies env.files 
+  ensures env.ok.ok() ==> env.constants.CommandLineArgs()[2] in env.files.state();
+  ensures env.constants.CommandLineArgs()[1] in env.files.state()
+  //ensures env.ok.ok()  ==> var copyname := env.constants.CommandLineArgs()[2];
+    //      old(env.files.state()) == env.files.state()[copyname:=[]];
+  ensures env.ok.ok() ==> copyFile(env.constants.CommandLineArgs()[1],env.constants.CommandLineArgs()[2],env); 
+  {
+   
+  var bufferSize:=0;
+  var sucessLen;
+  var original:= env.constants.GetCommandLineArg(1,env);    var copy :=env.constants.GetCommandLineArg(2,env);
+  sucessLen,bufferSize := FileStream.FileLength(original,env);
+  
+ 
+  var originalStream, copyStream;
+  var successOriginal,successCopy:=false,false;
+  var successRead,successWrite := false,false;
+   var successClose,successCloseCopy := false,false;
+  if(sucessLen){
+     var buffer := new  byte[bufferSize];
+  successOriginal,originalStream := FileStream.Open(original,env);
+   if(successOriginal){
+      successCopy,copyStream := FileStream.Open(copy,env);
+      if(successCopy){
+        successRead := originalStream.Read(0,buffer,0,bufferSize);
+        if(successRead){
+          successWrite := copyStream.Write(0,buffer,0,bufferSize);
+          if(successWrite){
+            successClose := originalStream.Close();
+           if(successClose){
+            successCloseCopy := copyStream.Close();
+           }
+          }
+        }
+      }
+    }
+  }
+  if(successCloseCopy){
+    print("DONE!");
+  }
+
+  } 
+  
+predicate copyFile(original : seq<char>,copy : seq<char>, env: HostEnvironment)
+reads env
+reads env.files
+requires env.files != null
+requires original in env.files.state()
+requires copy in env.files.state()
 {
-  //adicionar throw a erro caso não haja argumentos suficientes.
-  var orignal := HostConstants.GetCommandLineArg(1,env);
-  var copy := HostConstants.GetCommandLineArg(2,env);
-
-
-
-    print "done!\n";
+  env.files.state()[original] == env.files.state()[copy]
 }
+
